src/Reflection/Syntax.v
@@ -281,7 +281,7 @@ Global Arguments mapf_interp_flat_type {_ _ _} _ {t} _.
 Global Arguments interp_type_gen {_} _ _.
 Global Arguments interp_flat_type {_} _ _.
 Global Arguments interp_type_rel_pointwise {_} _ _ {_} _ _.
-Global Arguments interp_type_gen_rel_pointwise {_} _ _ {_} _ _.
+Global Arguments interp_type_gen_rel_pointwise {_ _} _ {_} _ _.
 Global Arguments interp_flat_type_rel_pointwise {_} _ _ {_} _ _.
 Global Arguments interp_type {_} _ _.
 Global Arguments wff {_ _ _ _ _} G {t} _ _.
